Contracts/Vault/Solidity.lean
@@ -1,7 +1,0 @@
-import Verity.Solidity
-
-namespace Contracts.Vault
-
-solidity_contract Solidity from "../../examples/solidity/Vault.sol"
-
-end Contracts.Vault
